teaching/taltech2018/sols_hidden/ex7/BinarySearchTreeClient.fst
@@ -1,0 +1,50 @@
+module BinarySearchTreeClient
+
+open FStar.ST
+
+open BinarySearchTree
+
+(* Client code to test mutable binary search trees in BinarySearchTree *)
+
+#set-options "--max_ifuel 0"
+
+let test_create_insert_search () : St unit =
+
+  let t1,r = create () in
+  let t2 = insert t1 r 0 in
+  let t3 = insert t2 r 1 in 
+  let t4 = insert t3 r 2 in 
+  let t5 = insert t4 r 0 in 
+    
+  let b1 = search t5 r 0 in
+  let b2 = search t5 r 2 in
+  let b3 = search t5 r 1 in
+  let b4 = search t5 r 3 in
+  
+  let t6 = insert t5 r 3 in 
+  let b5 = search t6 r 3 in
+  
+  let t1',r' = create () in
+  let b6 = search t1' r' 0 in
+  let t2' = insert t1' r' 4 in
+  let b7 = search t2' r' 4 in
+
+  let b8 = search t6 r 5 in
+  let t7 = insert t6 r 6 in 
+  let b9 = search t7 r 5 in
+  let b10 = search t7 r 6 in
+  let b11 = search t7 r 1 in 
+
+  assert (t4 == t5);
+
+  assert b1;
+  assert b2;
+  assert b3;
+  assert (not b4);
+  assert b5;
+  assert (not b6);
+  assert b7;
+  assert (not b8);
+  assert (not b9);
+  assert b10;
+  assert b11
